parse_varint

src/QUIC.Parse.fst
@@ -3,6 +3,310 @@ open FStar.HyperStack.ST
 
 open LowParse.Spec.BitSum
 
+(* From
+https://tools.ietf.org/html/draft-ietf-quic-transport-23#section-16,
+except that we make the format non-ambiguous. *)
+
+open LowParse.Spec.BoundedInt
+
+inline_for_extraction
+let parse_varint_payload_kind = {
+  parser_kind_low = 0;
+  parser_kind_high = Some 7;
+  parser_kind_subkind = Some ParserStrong;
+  parser_kind_metadata = None;
+}
+
+module Cast = FStar.Int.Cast
+module U64 = FStar.UInt64
+module U32 = FStar.UInt32
+module U16 = FStar.UInt16
+module U8 = FStar.UInt8
+
+inline_for_extraction
+let varint_bound : (varint_bound: U64.t { U64.v varint_bound == pow2 62 }) =
+  [@inline_let] let v = 4611686018427387904uL in
+  [@inline_let] let _ = assert_norm (U64.v v == pow2 62) in
+  v
+
+inline_for_extraction
+let varint_t = (x: U64.t { U64.v x < U64.v varint_bound })
+
+#push-options "--z3rlimit 32"
+
+inline_for_extraction
+let synth_u14
+  (msb: U64.t { U64.v msb < 64 })
+  (lsb: U8.t)
+: Tot varint_t
+= [@inline_let] let _ =
+    assert_norm (pow2 8 == 256);
+    assert (pow2 62 == U64.v varint_bound)
+  in
+  (msb `U64.mul` 256uL) `U64.add` Cast.uint8_to_uint64 lsb  
+
+let synth_u14_injective
+  (msb: U64.t { U64.v msb < 64 })
+: Lemma
+  (synth_injective (synth_u14 msb))
+  [SMTPat (synth_injective (synth_u14 msb))]
+= ()
+
+inline_for_extraction
+let synth_u30
+  (msb: U64.t { U64.v msb < 64 })
+  (lsb: bounded_integer 3)
+: Tot varint_t
+= [@inline_let] let _ =
+    assert_norm (pow2 8 == 256);
+    assert (pow2 62 == U64.v varint_bound);
+    assert_norm (pow2 24 == 16777216)
+   in
+   (msb `U64.mul` 16777216uL) `U64.add` Cast.uint32_to_uint64 lsb
+
+let synth_u30_injective
+  (msb: U64.t { U64.v msb < 64 })
+: Lemma
+  (synth_injective (synth_u30 msb))
+  [SMTPat (synth_injective (synth_u30 msb))]
+= ()
+
+inline_for_extraction
+let synth_u62
+  (msb: U64.t { U64.v msb < 64 })
+  (lsb: (U32.t & bounded_integer 3))
+: Tot varint_t
+= [@inline_let]
+  let (hi, lo) = lsb in
+  [@inline_let] let _ =
+    assert_norm (pow2 8 == 256);
+    assert (pow2 62 == U64.v varint_bound);
+    assert_norm (pow2 24 == 16777216);
+    assert_norm (pow2 32 == 4294967296)
+  in
+  Cast.uint32_to_uint64 lo `U64.add` (16777216uL `U64.mul` (Cast.uint32_to_uint64 hi `U64.add` (4294967296uL `U64.mul` msb)))
+
+let synth_u62_msb
+  (msb: U64.t { U64.v msb < 64 })
+  (lsb: (U32.t & bounded_integer 3))
+: Lemma
+  (U64.v (synth_u62 msb lsb) / 72057594037927936 == U64.v msb)
+= ()
+
+let synth_u62_injective
+  (msb: U64.t { U64.v msb < 64 })
+: Lemma
+  (synth_injective (synth_u62 msb))
+  [SMTPat (synth_injective (synth_u62 msb))]
+= ()
+
+inline_for_extraction
+let filter_u14
+  (y: varint_t)
+: Tot bool
+= 64uL `U64.lte` y
+
+inline_for_extraction
+let filter_u30
+  (y: varint_t)
+: Tot bool
+= 16384uL `U64.lte` y
+
+inline_for_extraction
+let filter_u62
+  (y: varint_t)
+: Tot bool
+= 1073741824uL `U64.lte` y
+    
+inline_for_extraction
+let id_u14
+  (y: parse_filter_refine filter_u14)
+: Tot varint_t
+= y
+
+let parse_varint_payload_u14
+  (msb: U64.t { U64.v msb < 64 })
+: Tot (parser parse_varint_payload_kind varint_t)
+= 
+  weaken parse_varint_payload_kind
+    (((parse_u8 `parse_synth` synth_u14 msb)
+    `parse_filter` filter_u14)
+    `parse_synth` id_u14)
+    
+inline_for_extraction
+let id_u30
+  (y: parse_filter_refine filter_u30)
+: Tot varint_t
+= y
+
+let parse_varint_payload_u30
+  (msb: U64.t { U64.v msb < 64 })
+: Tot (parser parse_varint_payload_kind varint_t)
+= 
+  weaken parse_varint_payload_kind
+    (((parse_bounded_integer 3 `parse_synth` synth_u30 msb)
+    `parse_filter` filter_u30)
+    `parse_synth` id_u30)
+
+inline_for_extraction
+let id_u62
+  (y: parse_filter_refine filter_u62)
+: Tot varint_t
+= y
+
+let parse_varint_payload_u62
+  (msb: U64.t { U64.v msb < 64 })
+: Tot (parser parse_varint_payload_kind varint_t)
+= 
+  weaken parse_varint_payload_kind
+    ((((parse_u32 `nondep_then` parse_bounded_integer 3) `parse_synth` synth_u62 msb)
+    `parse_filter` filter_u62)
+    `parse_synth` id_u62)
+
+let parse_varint_payload_14_interval
+  (msb: U64.t { U64.v msb < 64 })
+  (b: bytes)
+: Lemma
+  (requires (Some? (parse (parse_varint_payload_u14 msb) b)))
+  (ensures (
+    let Some (v, _) = parse (parse_varint_payload_u14 msb) b in
+    64 <= U64.v v /\
+    U64.v v < 16384 /\
+    U64.v msb == U64.v v / 256
+  ))
+= 
+   assert_norm (pow2 6 == 64);
+   assert_norm (pow2 8 == 256);
+   assert (pow2 62 == U64.v varint_bound);
+   assert_norm (pow2 32 == 4294967296);
+   assert_norm (pow2 24 == 16777216);
+   parse_synth_eq parse_u8 (synth_u14 msb) b;
+   parse_filter_eq (parse_u8 `parse_synth` (synth_u14 msb)) filter_u14 b;
+   parse_synth_eq ((parse_u8 `parse_synth` (synth_u14 msb)) `parse_filter` filter_u14) id_u14 b
+
+let parse_varint_payload_30_interval
+  (msb: U64.t { U64.v msb < 64 })
+  (b: bytes)
+: Lemma
+  (requires (Some? (parse (parse_varint_payload_u30 msb) b)))
+  (ensures (
+    let Some (v, _) = parse (parse_varint_payload_u30 msb) b in
+    16384 <= U64.v v /\
+    U64.v v < 1073741824 /\
+    U64.v msb == U64.v v / 16777216
+  ))
+= 
+    parse_synth_eq (parse_bounded_integer 3) (synth_u30 msb) b;
+    parse_filter_eq (parse_bounded_integer 3 `parse_synth` (synth_u30 msb)) filter_u30 b;
+    parse_synth_eq ((parse_bounded_integer 3 `parse_synth` (synth_u30 msb)) `parse_filter` filter_u30) (id_u30) b
+
+let parse_varint_payload_62_interval
+  (msb: U64.t { U64.v msb < 64 })
+  (b: bytes)
+: Lemma
+  (requires (Some? (parse (parse_varint_payload_u62 msb) b)))
+  (ensures (
+    let Some (v, _) = parse (parse_varint_payload_u62 msb) b in
+    1073741824 <= U64.v v /\
+    U64.v msb == U64.v v / (72057594037927936)
+  ))
+= 
+   assert_norm (pow2 6 == 64);
+   assert_norm (pow2 8 == 256);
+   assert (pow2 62 == U64.v varint_bound);
+   assert_norm (pow2 32 == 4294967296);
+   assert_norm (pow2 24 == 16777216);
+   parse_synth_eq (parse_u32 `nondep_then` parse_bounded_integer 3) (synth_u62 msb) b;
+   parse_filter_eq ((parse_u32 `nondep_then` parse_bounded_integer 3) `parse_synth` synth_u62 msb) filter_u62 b;
+   parse_synth_eq (((parse_u32 `nondep_then` parse_bounded_integer 3) `parse_synth` (synth_u62 msb)) `parse_filter` filter_u62) (id_u62) b;
+   let Some (v, _) = parse (parse_varint_payload_u62 msb) b in
+   let Some (lsb, _) = parse (parse_u32 `nondep_then` parse_bounded_integer 3) b in
+   synth_u62_msb msb lsb
+
+let parse_varint_payload
+  (x: U8.t)
+: Tot (parser parse_varint_payload_kind varint_t)
+= assert_norm (pow2 6 == 64);
+  assert_norm (pow2 8 == 256);
+  assert (pow2 62 == U64.v varint_bound);
+  assert_norm (pow2 32 == 4294967296);
+  assert_norm (pow2 24 == 16777216);
+  let kd = uint8.get_bitfield x 6 8 in
+  let msb = Cast.uint8_to_uint64 (uint8.get_bitfield x 0 6) in
+  if kd = 0uy
+  then weaken parse_varint_payload_kind (parse_ret msb)
+  else if kd = 1uy
+  then parse_varint_payload_u14 msb
+  else if kd = 2uy
+  then parse_varint_payload_u30 msb
+  else parse_varint_payload_u62 msb
+
+module BF = LowParse.BitFields
+
+let parse_varint_payload_interval
+  (tag: U8.t)
+  (b: bytes)
+: Lemma
+  (requires (Some? (parse (parse_varint_payload tag) b)))
+  (ensures (
+    let Some (v, _) = parse (parse_varint_payload tag) b in
+    let kd = uint8.get_bitfield tag 6 8 in
+    let msb = uint8.get_bitfield tag 0 6 in
+    (kd == 0uy \/ kd == 1uy \/ kd == 2uy \/ kd == 3uy) /\ (
+    if kd = 0uy
+    then U64.v v < 64 /\ U8.v msb = U64.v v
+    else if kd = 1uy
+    then 64 <= U64.v v /\ U64.v v < 16384 /\ U8.v msb == U64.v v / 256
+    else if kd = 2uy
+    then 16384 <= U64.v v /\ U64.v v < 1073741824 /\ U8.v msb == U64.v v / 16777216
+    else 1073741824 <= U64.v v /\ U8.v msb == U64.v v / 72057594037927936
+  )))
+=
+  assert_norm (pow2 6 == 64);
+  assert_norm (pow2 8 == 256);
+  assert (pow2 62 == U64.v varint_bound);
+  assert_norm (pow2 32 == 4294967296);
+  assert_norm (pow2 24 == 16777216);
+  let Some (v, _) = parse (parse_varint_payload tag) b in
+  let kd = uint8.get_bitfield tag 6 8 in
+  assert (kd == 0uy \/ kd == 1uy \/ kd == 2uy \/ kd == 3uy);
+  let msb8 = uint8.get_bitfield tag 0 6 in
+  let msb = Cast.uint8_to_uint64 msb8 in
+  if kd = 0uy
+  then begin
+    assert (U64.v v < 64);
+    assert (U8.v msb8 == U64.v v)
+  end
+  else if kd = 1uy
+  then begin
+    parse_varint_payload_14_interval msb b
+  end else if kd = 2uy
+  then
+    parse_varint_payload_30_interval msb b
+  else
+    parse_varint_payload_62_interval msb b
+
+#pop-options
+
+let parse_varint_payload_and_then_cases_injective : squash (and_then_cases_injective parse_varint_payload) =
+  assert_norm (pow2 8 == 256);
+  assert (pow2 62 == U64.v varint_bound);
+  assert_norm (pow2 32 == 4294967296);
+  assert_norm (pow2 24 == 16777216);
+  and_then_cases_injective_intro parse_varint_payload (fun x1 x2 b1 b2 ->
+    let msb1 = Cast.uint8_to_uint64 (uint8.get_bitfield x1 0 6) in
+    let msb2 = Cast.uint8_to_uint64 (uint8.get_bitfield x2 0 6) in
+    parse_varint_payload_interval x1 b1;
+    parse_varint_payload_interval x2 b2;
+    assert (uint8.v (uint8.get_bitfield x1 6 8) == uint8.v (uint8.get_bitfield x2 6 8));
+    assert (uint8.v (uint8.get_bitfield x1 0 6) == uint8.v (uint8.get_bitfield x2 0 6));
+    BF.get_bitfield_partition_2 6 (U8.v x1) (U8.v x2)
+  )
+
+let parse_varint : parser _ varint_t =
+  parse_u8 `and_then` parse_varint_payload
+
+
 (* From https://tools.ietf.org/html/draft-ietf-quic-transport-23#section-17 *)
 
 inline_for_extraction
@@ -50,8 +354,6 @@ noextract
 let reserved_bits : enum unit (bitfield uint8 2) = [
   (), 0uy;
 ]
-
-open LowParse.Spec.BoundedInt
 
 inline_for_extraction
 noextract
@@ -195,8 +497,6 @@ noextract
 let common_long_t
 : Type0
 = (FB.lbytes 4 & (parse_bounded_vlbytes_t 0 20 & parse_bounded_vlbytes_t 0 20))
-
-module U32 = FStar.UInt32
 
 #push-options "--z3rlimit 16 --max_fuel 8 --max_ifuel 8 --initial_fuel 8 --initial_ifuel 8"
 
